examples/robots/robots-prob.pddl
@@ -1,0 +1,21 @@
+
+
+(define (problem rb)
+    (:domain robots)
+    (:objects 
+        r1 r2 - robot 
+        b - block 
+        d - door 
+        rm1 rm2 - room)   
+    (:init 
+        (connects d rm1 rm2) 
+        (connects d rm2 rm1)
+        (in-room r1 rm1)
+        (in-room r2 rm2)
+        (in-room b rm1)
+        (idle r1) 
+        (idle r2)
+    )
+    (:goal (and (in-room b rm2)))
+)
+
